DTLC2 prove determinstic and an unhalting example

DTLC2.v
@@ -5,24 +5,24 @@ Require Import Coq.Strings.Ascii.
 
 
 
-Inductive _Exp : Set :=
-| _Const : id -> _Exp
-| _Var : id -> _Exp
-| _Lamb : id  -> _Exp -> _Exp
-| _Add : _Exp -> _Exp -> _Exp
-| _Minus : _Exp -> _Exp -> _Exp
-| _Mult : _Exp -> _Exp -> _Exp
-| _Apply : _Exp -> _Exp -> _Exp.
-
-
 Inductive _obj : Set :=
 | _int :  Z -> _obj
 | _str : string -> _obj
 | _list : list _obj -> _obj
 | _quote : string -> _obj
 | _quoteq : _obj -> _obj
-| _func : id -> _Exp -> _obj
 | _undef : _obj.
+
+
+Inductive _Exp : Set :=
+| _Const : _obj -> _Exp
+| _Var : id -> _Exp
+| _Lamb : id  -> _Exp -> _Exp
+| _ITNOp : _Exp -> _Exp -> _Exp
+| _Apply : _Exp -> _Exp -> _Exp.
+
+
+
 
 Definition _State := total_map _obj.
 
@@ -63,20 +63,71 @@ Fixpoint eval_ (st: _State) (exp : _Exp) {struct exp} : _obj :=
   end.*)
 
 
-Fixpoint substt (exp : _Exp) (var : _Exp) (bdd : _Exp) : _Exp :=
-  match exp with
-    | 
 
-Reserved Notation "exp '/' st1 '\\' st2 '/' val"
-         (at level 40, st1, st2 at level 39).
+Definition substt (var :_Exp) : _Exp -> _Exp -> {s| var = _Var s} -> _Exp.
+  refine (fix substt bdd exp h :=
+          match exp with
+            | _Const i => _Const i
+            | _Var i => match h with exist s P =>
+                                     match eq_id_dec i s with
+                                       | left h1 => bdd
+                                       | right h2 => _Var i
+                                     end
+                        end
+            | _Lamb i exp' => match h with exist s P =>
+                                           match eq_id_dec i s with
+                                             | left h1 => _Lamb i exp'
+                                             | right h2 => _Lamb i (substt bdd exp' h)
+                                           end
+                              end
+                                                               
+            | _ITNOp exp1 exp2 => _ITNOp (substt bdd exp1 h) (substt bdd exp2 h)
+            | _Apply func arg => _Apply (substt bdd func h) (substt bdd arg h)
+          end).
+Defined.
 
-Inductive SevalR : _Exp -> _State -> _State -> _obj -> Prop :=
-| e_const : forall v x st, st x = v ->  (_Const x) / st \\ st / v
-| e_var : forall v x st, st x = v -> (_Var x) / st \\ st / v
-| e_Lam : forall i st exp, (_Lamb i exp) / st \\ st / _func i exp
-| e_App : forall i st v argExp funExp bodyexp v' , 
-            (argExp / st \\ st / v) ->
-            (funExp / st \\ st / (_func i bodyexp)) ->
-            (bodyexp / (t_update st i v) \\ (t_update st i v) / v') ->
-            (_Apply funExp argExp) / st \\ st / v'
-where "exp '/' st1 '\\' st2 '/' val" := (SevalR exp st1 st2 val).
+
+Reserved Notation "exp '\\' val"
+         (at level 40).
+
+Inductive SevalR : _Exp -> _Exp -> Prop :=
+| e_const : forall x, (_Const x) \\ (_Const x)
+| e_Lam : forall exp i, (_Lamb i exp) \\  (_Lamb i exp)
+| e_App : forall argExp funExp bodyExp i v1 v2 , 
+            (argExp  \\ v1) ->
+            (funExp \\ (_Lamb i bodyExp)) ->
+            (substt (_Var i) v1 bodyExp (exist _ i eq_refl) \\ v2) ->
+            (_Apply funExp argExp) \\ v2
+where "exp '\\' val" := (SevalR exp val).
+
+Theorem DTLC_determine:
+  forall exp v1 v2,
+    exp \\ v1 -> exp \\ v2 -> v1 = v2.
+  intros exp v1 v2 h1; generalize v2; clear v2.
+  elim h1; try(intros; inversion H; auto).
+  subst v0. subst argExp. inversion H5. pose (H0 _ H8). rewrite <- e in H11. pose (H2 _ H9).
+  inversion e0. subst bodyExp0. subst i. auto. inversion H5. pose (H0 _ H10). pose (H2 _ H11).
+  inversion e0. subst bodyExp0. symmetry in e. subst v4. subst i1. auto.
+  inversion H5. pose(H0 _ H13). pose (H2 _ H14). inversion e0. symmetry in e. subst v6; subst bodyExp1. subst i1. auto.
+Qed.
+
+
+
+Definition part_unhalting:=
+  _Lamb (Id 1) (_Apply (_Var (Id 1)) (_Var (Id 1))).
+
+Definition unhalting := _Apply part_unhalting part_unhalting.
+
+
+
+Lemma classic_unhalting:
+  forall v, ~ (unhalting \\ v).
+  unfold not. intros.
+  remember unhalting as c.
+  generalize Heqc. elim H; try (intros; subst c; discriminate).
+  intros. unfold unhalting in Heqc0. inversion Heqc0.
+  subst funExp. unfold part_unhalting in H2. inversion H2. rewrite H10 in H11.
+  subst bodyExp. inversion Heqc0. subst argExp. inversion H0. fold part_unhalting in H6.
+  simpl in H5. simpl in H4. rewrite eq_id_dec_id in H5. subst v1. fold unhalting in H5. auto.
+Qed.
+
