Imp.v
@@ -570,4 +570,8 @@ Qed.
     intros. inversion Heqc0. rewrite H2 in H0. simpl in H0. inversion H0.
   Qed.
 
-  
+    Theorem loop_never_stops___:
+    forall st st', ~(loop / st \\ st').
+      unfold loop. unfold not.
+      intros. remember (WHILE BTrue DO SKIP END) as c.
+      generalize Heqc. elim H
